Rename vrel to nrel

aeq/type.lean
@@ -8,20 +8,20 @@ we want Lean to cache the results.
 -/
 
 import exp
-import vrel
+import nrel
 
 open [notation] finset
-open [notation] vrel
+open [notation] nrel
 
 -- `V` is the type of an infinite set of variable names with decidable equality.
 variables {V : Type} [decidable_eq V]
 
 /-
 `aeq R e₁ e₂` is an inductive data type that relates `e₁ : exp X` and `e₂ : exp
-Y` via their free variables with `R : vrel X`.
+Y` via their free variables with `R : nrel X`.
 -/
 
-inductive aeq : Π {X Y : finset V}, vrel X Y → exp X → exp Y → Prop :=
-  | var : Π {X Y : finset V} {R : vrel X Y}           {x : ν∈ X}            {y : ν∈ Y},            ⟪x, y, R⟫ →                     aeq R (exp.var x)     (exp.var y)
-  | app : Π {X Y : finset V} {R : vrel X Y}           {fX eX : exp X}       {fY eY : exp Y},       aeq R fX fY → aeq R eX eY →     aeq R (exp.app fX eX) (exp.app fY eY)
-  | lam : Π {X Y : finset V} {R : vrel X Y} {a b : V} {eX : exp ('{a} ∪ X)} {eY : exp ('{b} ∪ Y)}, aeq (vrel.update a b R) eX eY → aeq R (exp.lam eX)    (exp.lam eY)
+inductive aeq : Π {X Y : finset V}, nrel X Y → exp X → exp Y → Prop :=
+  | var : Π {X Y : finset V} {R : nrel X Y}           {x : ν∈ X}            {y : ν∈ Y},            ⟪x, y, R⟫ →                     aeq R (exp.var x)     (exp.var y)
+  | app : Π {X Y : finset V} {R : nrel X Y}           {fX eX : exp X}       {fY eY : exp Y},       aeq R fX fY → aeq R eX eY →     aeq R (exp.app fX eX) (exp.app fY eY)
+  | lam : Π {X Y : finset V} {R : nrel X Y} {a b : V} {eX : exp ('{a} ∪ X)} {eY : exp ('{b} ∪ Y)}, aeq (nrel.update a b R) eX eY → aeq R (exp.lam eX)    (exp.lam eY)
