aeq/map.lean
@@ -10,19 +10,19 @@ open [notation] eq.ops
 open [notation] finset
 open [notation] function
 open [notation] sigma.ops
-open [notation] vrel
+open [notation] nrel
 
 -- `V` is the type of an infinite set of variable names with decidable equality.
 variables {V : Type} [decidable_eq V]
 
 namespace aeq -- ===============================================================
 
-variables {X₁ Y₁ : finset V} {R : vrel X₁ Y₁} {eX : exp X₁} {eY : exp Y₁}
+variables {X₁ Y₁ : finset V} {R : nrel X₁ Y₁} {eX : exp X₁} {eY : exp Y₁}
 
 -- The `map` implementation for `aeq`.
 lemma map_core (H : aeq R eX eY)
 : ∀ {X₂ Y₂ : finset V} (pX : X₁ ⊆ X₂) (pY : Y₁ ⊆ Y₂)
-    {S : vrel X₂ Y₂} (F : vrel.translate R S)
+    {S : nrel X₂ Y₂} (F : nrel.translate R S)
 , aeq S (exp.map pX eX) (exp.map pY eY) :=
 
   begin
@@ -44,16 +44,16 @@ lemma map_core (H : aeq R eX eY)
       exact lam $
         r (finset.insert_subset_insert x pX)
           (finset.insert_subset_insert y pY)
-          (λ x y, vrel.translate_update @F)
+          (λ x y, nrel.translate_update @F)
     end
   end
 
-variables {X₂ Y₂ : finset V} {S : vrel X₂ Y₂}
+variables {X₂ Y₂ : finset V} {S : nrel X₂ Y₂}
 
--- Map alpha-equality from one variable relation, `R : vrel X₁ Y₁`, to another,
--- `S : vrel X₂ Y₂`, as long as `X₁ ⊆ X₂` and `Y₁ ⊆ Y₂`.
+-- Map alpha-equality from one variable relation, `R : nrel X₁ Y₁`, to another,
+-- `S : nrel X₂ Y₂`, as long as `X₁ ⊆ X₂` and `Y₁ ⊆ Y₂`.
 theorem map (pX : X₁ ⊆ X₂) (pY : Y₁ ⊆ Y₂)
-: vrel.translate R S → aeq R eX eY → aeq S (exp.map pX eX) (exp.map pY eY) :=
+: nrel.translate R S → aeq R eX eY → aeq S (exp.map pX eX) (exp.map pY eY) :=
 
   λ F H, map_core H pX pY @F
 
@@ -61,14 +61,14 @@ end aeq -- namespace -----------------------------------------------------------
 
 namespace aeq -- ===============================================================
 
-variables {X Y : finset V} {R S : vrel X Y} {eX : exp X} {eY : exp Y}
+variables {X Y : finset V} {R S : nrel X Y} {eX : exp X} {eY : exp Y}
 
 -- A wrapper for `map` in which the free variable sets do not change.
 theorem map_simple
 : (∀ {x : ν∈ X} {y : ν∈ Y}, ⟪x, y, R⟫ → ⟪x, y, S⟫) → aeq R eX eY → aeq S eX eY :=
 
   assume F H,
-  have F' : vrel.translate R S, by apply vrel.translate_simple; apply @F,
+  have F' : nrel.translate R S, by apply nrel.translate_simple; apply @F,
   exp.eq_of_map X eX ▸ exp.eq_of_map Y eY ▸
     map (finset.subset.refl X) (finset.subset.refl Y) @F' H
 
