nrel/core.lean
@@ -1,6 +1,6 @@
 /-
 
-This files contains a collection of core definitions and properties for `vrel`.
+This files contains a collection of core definitions and properties for `nrel`.
 
 -/
 
@@ -15,50 +15,50 @@ variables {V : Type} [decidable_eq V]
 -- `X`, `Y`, and `Z` are finite sets of variable names.
 variables {X Y Z : finset V}
 
-namespace vrel -- ==============================================================
--- We define the core operations on `vrel`.
+namespace nrel -- ==============================================================
+-- We define the core operations on `nrel`.
 
--- `mem` is a synonym for the function defined by `vrel` applied to arguments.
-definition mem (x : ν∈ X) (y : ν∈ Y) (R : vrel X Y) : Prop :=
+-- `mem` is a synonym for the function defined by `nrel` applied to arguments.
+definition mem (x : ν∈ X) (y : ν∈ Y) (R : nrel X Y) : Prop :=
   R x y
 
--- Convenient notation for `mem`.
+-- notation for `mem`.
 notation `⟪` x `, ` y `, ` R `⟫` := mem x y R
 notation `⟪` R `⟫` := mem _ _ R  -- if the member properties can be inferred
 
 -- `id X` creates an identity variable relation from the single finite set `X`.
-definition id (X : finset V) : vrel X X :=
+definition id (X : finset V) : nrel X X :=
   eq
 
 -- `inverse R` inverts the order of the relation `R`.
-definition inverse : vrel X Y → vrel Y X :=
+definition inverse : nrel X Y → nrel Y X :=
   function.swap
 
 -- `compose R S` combines the relations `R` and `S` to create a new relation
 -- that is the composition of their underlying finite sets.
-definition compose (R : vrel X Y) (S : vrel Y Z) : vrel X Z :=
+definition compose (R : nrel X Y) (S : nrel Y Z) : nrel X Z :=
   λ x z, ∃ y, R x y ∧ S y z
 
--- Convenient notation for `compose`.
+-- Notation for `compose`.
 -- Source: http://www.fileformat.info/info/unicode/char/2a3e/index.htm
 notation R ` ⨾ `:60 S := compose R S
 
--- Lift a function to a `vrel`
-definition lift (F : ν∈ X → ν∈ Y) : vrel X Y :=
+-- Lift a function to a `nrel`
+definition lift (F : ν∈ X → ν∈ Y) : nrel X Y :=
   λ x y, (F x).1 = y.1
 
-end vrel -- namespace ----------------------------------------------------------
+end nrel -- namespace ----------------------------------------------------------
 
 -- Global attributes
-attribute vrel.mem     [reducible]
-attribute vrel.id      [reducible]
-attribute vrel.inverse [reducible]
-attribute vrel.compose [reducible]
+attribute nrel.mem     [reducible]
+attribute nrel.id      [reducible]
+attribute nrel.inverse [reducible]
+attribute nrel.compose [reducible]
 
-namespace vrel -- ==============================================================
+namespace nrel -- ==============================================================
 -- These are basic properties of the above definitions.
 
-variables {R : vrel X Y} {S : vrel Y Z}
+variables {R : nrel X Y} {S : nrel Y Z}
 
 theorem mem_id : ∀ (x : ν∈ X), ⟪x, x, id X⟫ :=
   eq.refl
@@ -71,9 +71,9 @@ theorem mem_compose : ⟪x, y, R⟫ → ⟪y, z, S⟫ → ⟪x, z, R ⨾ S⟫ :=
 theorem mem_inverse_iff_mem : (⟪x, y, R⟫ ↔ ⟪y, x, inverse R⟫) :=
   iff.intro (λ H, H) (λ H, H)
 
-end vrel -- namespace ----------------------------------------------------------
+end nrel -- namespace ----------------------------------------------------------
 
-namespace vrel -- ==============================================================
+namespace nrel -- ==============================================================
 -- These are properties on `id X` relations.
 
 variables {x₁ x₂ x₃ : ν∈ X}
@@ -91,4 +91,4 @@ theorem mem_id_of_mem_compose_id : ⟪x₁, x₃, id X ⨾ id X⟫ ↔ ⟪x₁, 
     exists.intro x₁ (and.intro rfl H),
   iff.intro (by assumption) (by assumption)
 
-end vrel -- namespace ----------------------------------------------------------
+end nrel -- namespace ----------------------------------------------------------
