nrel/type.lean
@@ -1,0 +1,20 @@
+/-
+
+This file contains the `nrel` type, a binary relation on finite sets of
+variable names.
+
+-/
+
+import name
+
+-- `V` is the type of an infinite set of variable names with decidable equality.
+variables {V : Type} [decidable_eq V]
+
+/-
+`nrel` is the type of a binary relation on finite sets of variable names. It is
+defined by a function on two variable names in their respective finite sets `X`
+and `Y`.
+-/
+
+definition nrel (X Y : finset V) : Type :=
+  ν∈ X → ν∈ Y → Prop
